\section{Given the following grammar specification, draw the corresponding parse tree and write a leftmost derivation for each of the following statements.}
\begin{align*}
<assignment> &\mapsto <identifier> = <expression> \\
<identifier> &\mapsto A \\ 
&\mapsto B \\ 
&\mapsto C \\ 
<expression> &\mapsto <identifier> + <expression> \\
&\mapsto <identifier> * <expression> \\
&\mapsto (<expression>) \\
&\mapsto <identifier> \\
\end{align*}
\paragraph{Explanation of the problem}
we are going to expanded out the statement in the context of the grammar to show all of its derivations in both the text format in the \textbf{leftmost} derivation, and the graphical format of the \textbf{parse tree}. 
\subsection{\(A=A*(B+(C*A))\)}
\subsubsection{Leftmost Derivation}
\begin{align*}
<assignment> &\mapsto <identifier> = <expression> \\
&\mapsto A = <expression> \\
&\mapsto A = <identifier> * <expression> \\
&\mapsto A = A * <expression> \\
&\mapsto A = A * (<expression>) \\
&\mapsto A = A * (<identifier> + <expression>)\\
&\mapsto A = A * (B + <expression>)\\
&\mapsto A = A * (B + (<expression>))\\
&\mapsto A = A * (B + (<identifier> * <expression>))\\
&\mapsto A = A * (B + (C * <expression>))\\
&\mapsto A = A * (B + (C * <identifier>))\\
&\mapsto A = A * (B + (C * A))\\
\end{align*}
\subsubsection{Parse Tree}

\begin{forest}
where n children=0{tier=word}{}
	[assignment[id[A]][{=}][expression
	[identifier[A]][{*}][expression
		[{(expression)}
			[identifier[(B]][{+}][expression
				[{(expression)}
					[identifier[(C]][{*}][expression[identifier[A)]]]]]]]
]]
\end{forest}
\subsection{\(B=C*(A*C+B)\)}
\subsubsection{Leftmost Derivation}
\begin{align*}
<assignment> &\mapsto <identifier> = <expression> \\
&\mapsto B = <expression> \\
&\mapsto B = <identifier> * <expression> \\
&\mapsto B = C * <expression> \\
&\mapsto B = C * (<expression>) \\
&\mapsto B = C * (<identifier> * <expression>) \\
&\mapsto B = C * (A * <expression>) \\
&\mapsto B = C * (A * <identifier> + <expression>)) \\
&\mapsto B = C * (A * C + <expression>)) \\
&\mapsto B = C * (A * C + <identifier>)) \\
&\mapsto B = C * (A * C + B)) \\
\end{align*}
\subsubsection{Parse Tree}
\begin{forest}
where n children=0{tier=word}{}
	[assignment
		[identifier[B]][{=}][expression
			[identifier[C]][{*}][expression[(expression)
				[identifier[(A]][{*}][expression
				]]
				[(expression)
				[identifier[C]][{+}][expression[identifier[B)]]]]
				]]]
\end{forest}
